\documentclass[11pt]{article}

\usepackage[margin=1.25in]{geometry}

\usepackage{amsmath}
\usepackage{amssymb}
\usepackage{graphicx}
\usepackage{amsfonts}
\usepackage{braket}
\usepackage{enumitem}

\usepackage{tikz}
\usetikzlibrary{calc}
\usepackage{calculator}
\usepackage{standalone}



\begin{document}

\title{Particle Gravitation}
\author{Gabriele Carcassi, Christine A. Aidala}


%\ifjournal
%	% As the page margins are so large, the full title does not fit
%	\titlerunning{From physical principles to classical and quantum particle mechanics}
%\fi

\date{\today}

\maketitle

\begin{abstract}
\end{abstract}

\tableofcontents
\newpage

\section{General properties}
\begin{equation}
\begin{aligned}
a \wedge b &= a \otimes b - b \otimes a \\
g_{\alpha\beta} e^\alpha \wedge e^\beta &= g_{\alpha\beta} e^\alpha \otimes e^\beta - g_{\alpha\beta} e^\beta \otimes e^\alpha = g_{\alpha\beta} e^\alpha \otimes e^\beta - g_{\beta\alpha} e^\alpha \otimes e^\beta \\
&= (g_{\alpha\beta} - g_{\beta\alpha}) e^\alpha \otimes e^\beta \\
\end{aligned}
\end{equation}
\begin{equation}
\begin{aligned}
\partial_\alpha \delta^\beta_\gamma &= 0 = \partial_\alpha ( g^{\beta \delta} g_{\delta \gamma} ) = \partial_\alpha g^{\beta \delta} g_{\delta \gamma} + g^{\beta \delta} \partial_\alpha g_{\delta \gamma} \\
\partial_\alpha g^{\beta \gamma} &= - g^{\beta \delta} g^{\gamma \epsilon} \partial_\alpha g_{\delta \epsilon} \\
\Gamma_{\alpha \beta \gamma} &= (\partial_\gamma g_{\alpha\beta} + \partial_\beta g_{\alpha\gamma} - \partial_\alpha g_{\beta\gamma}) \\
\Gamma^\alpha_{\beta\gamma} &= g^{\alpha \delta} \Gamma_{\delta\beta\gamma}
\end{aligned}
\end{equation}

\section{Position and conjugate momentum}

\begin{equation}
\begin{aligned}
\theta &= \left[ \begin{matrix}
p_\alpha & 0 \end{matrix} \right] \\
\theta &= \theta_a e^a = p_\alpha e^{q^\alpha} \\
\omega &= - \partial \theta = - \partial_b \theta_a e^b \wedge e^a = - e^{p_\alpha} \wedge e^{q^\alpha}  \\
\omega &= \left[ \begin{matrix}
0 & I_n \\[2.2ex]
- I_n & 0 \end{matrix} \right] \\
\omega &= \omega_{ab} e^a \otimes e^b = e^{q^\alpha} \otimes e^{p_\alpha} - e^{p_\alpha} \otimes e^{q^\alpha} = e^{q^\alpha} \wedge e^{p_\alpha} \\
\end{aligned}
\end{equation}

\section{Position and kinetic momentum}
\begin{equation}
\begin{aligned}
	d\xi^a \omega_{ab} d\xi^b &= dq^\alpha dp_\alpha = dx^\alpha g_{\alpha\beta} du^\beta \\
	q^\alpha &= x^\alpha \\
	p_\alpha &= m g_{\alpha \beta} u^\beta + q A_\alpha \\
	&= \Pi_\alpha + q A_\alpha \\
	\Pi_\alpha &= m g_{\alpha \beta} u^\beta \\
	&= dq^i dp_i - dt dE \\
	\mathcal{H} &= \frac{1}{2m} \Pi_\alpha g^{\alpha\beta} \Pi_\beta 
\end{aligned}
\end{equation}
\begin{equation}
\begin{aligned}
	e^{q^\alpha} &= \frac{\partial q^\alpha}{\partial x^\beta}e^{x^\beta} + \frac{\partial q^\alpha}{\partial \Pi_\gamma}e^{\Pi_\gamma} = e^{x^\alpha} \\
	e^{p_\alpha} &= \frac{\partial p_\alpha}{\partial x^\beta}e^{x^\beta} + \frac{\partial p_\alpha}{\partial \Pi_\gamma}e^{\Pi_\gamma} \\
	&= q \frac{\partial A_\alpha}{\partial x^\beta} e^{x^\beta} +e^{\Pi_\alpha} \\
\end{aligned}
\end{equation}
\begin{equation}
\begin{aligned}
	\theta &= (\Pi_\alpha + q A_\alpha) e^{x^\alpha} \\
	\omega &= e^{x^\alpha} \wedge \left( q \frac{\partial A_\alpha}{\partial x^\beta} e^{x^\beta} +e^{\Pi_\alpha} \right) \\
	&= q \frac{\partial A_\alpha}{\partial x^\beta} e^{x^\alpha} \wedge e^{x^\beta} + e^{x^\alpha} \wedge e^{\Pi_\alpha} \\
	&=  q \left( \frac{\partial A_\alpha}{\partial x^\beta} - \frac{\partial A_\beta}{\partial x^\alpha}\right)  e^{x^\alpha} \otimes e^{x^\beta} \\
	&+ e^{x^\alpha} \otimes e^{\Pi_\gamma} - e^{\Pi_\gamma} \otimes e^{x^\alpha} \\
	F_{\alpha\beta} &= \partial_\alpha A_\beta - \partial_\beta A_\alpha \\
	\omega_{ab} &= \left[ \begin{matrix}
		- q F_{\alpha\beta} & I_n \\[2.2ex]
		- I_n & 0 \end{matrix} \right] \\
\end{aligned}
\end{equation}
\begin{equation}
\begin{aligned}
e_{q^\alpha} &= \frac{\partial x^\beta }{\partial q^\alpha}e_{x^\beta} + \frac{\partial \Pi_\beta}{\partial q^\alpha}e_{\Pi_\beta} \\
&= e_{x^\alpha} - q \frac{\partial A_\beta}{\partial q^\alpha}e_{\Pi_\beta} \\
e_{p_\alpha} &= \frac{\partial x^\beta}{\partial p_\alpha}e_{x^\beta} + \frac{\partial \Pi_\gamma}{\partial p_\alpha}e_{\Pi_\gamma} \\
&= e_{\Pi_\alpha} \\
\end{aligned}
\end{equation}
\begin{equation}
\begin{aligned}
\{x^\alpha, x^\beta\} &= \{q^\alpha, q^\beta\} = 0 \\
\{x^\alpha, \Pi_\beta\} &= \{q^\alpha, p_\beta - q A_\beta\} = \{q^\alpha, p_\beta\} - \{q^\alpha, q A_\beta\} \\
\{f(x^\alpha), \Pi_\beta\} &= \{f(q^\alpha), p_\beta - q A_\beta\} = \{f(q^\alpha), p_\beta\} - \{f(q^\alpha), q A_\beta\} \\
&= \partial_\beta f(q^\alpha) \\
\{ \Pi_\alpha, \Pi_\beta\} &= \{p_\alpha - q A_\alpha, p_\beta - q A_\beta\} \\
&= \{p_\alpha, p_\beta\} - \{p_\alpha, q A_\beta\} - \{q A_\alpha, p_\beta\} + \{q A_\alpha , q A_\beta\} \\
&= \{q A_\beta, p_\alpha\} - \{q A_\alpha, p_\beta\} = q (\partial_\alpha A_\beta - \partial_\beta A_\alpha) \\
&= q F_{\alpha \beta} \\
\end{aligned}
\end{equation}
\begin{equation}
\begin{aligned}
d_s x^\alpha = \{x^\alpha, \mathcal{H}\} &= \frac{1}{2m} \{x^\alpha, \Pi_\beta g^{\beta\gamma} \Pi_\gamma\} = \frac{1}{m} g^{\alpha \beta} \Pi_\beta \\
m g_{\alpha\beta} d_s x^\beta &= \Pi_\alpha \\
d_s \Pi_\alpha = \{ \Pi_\alpha , \mathcal{H} \} &= \frac{1}{2m} \{\Pi_\alpha, \Pi_\beta g^{\beta\gamma} \Pi_\gamma\} \\
&= \frac{1}{2m} \left( \{\Pi_\alpha, \Pi_\beta\}  g^{\beta\gamma} \Pi_\gamma + \{\Pi_\alpha,  g^{\beta\gamma} \} \Pi_\beta \Pi_\gamma + \{\Pi_\alpha,  \Pi_\gamma\} \Pi_\beta g^{\beta\gamma} \right)  \\
&= \frac{1}{2m} \left( q F_{\alpha \beta}  g^{\beta\gamma} \Pi_\gamma - \partial_\alpha g^{\beta\gamma} \Pi_\beta \Pi_\gamma + q F_{\alpha \gamma} \Pi_\beta g^{\beta\gamma} \right)  \\
&= - \frac{1}{2m} \partial_\alpha g^{\beta\gamma} \Pi_\beta \Pi_\gamma + \frac{q}{m} F_{\alpha\beta} g^{\beta\gamma} \Pi_\gamma \\
&= \frac{1}{2m} g^{\beta\delta} g^{\gamma\epsilon} \partial_\alpha g_{\delta\epsilon} \Pi_\beta \Pi_\gamma + \frac{q}{m} F_{\alpha\beta} g^{\beta\gamma} \Pi_\gamma \\
&= \frac{1}{2m} g^{\beta\delta} g^{\gamma\epsilon}(\partial_\epsilon g_{\delta\alpha} - \partial_\epsilon g_{\delta\alpha} + \partial_\alpha g_{\delta\epsilon} ) \Pi_\beta \Pi_\gamma + \frac{q}{m} F_{\alpha\beta} g^{\beta\gamma} \Pi_\gamma \\
&= \frac{1}{2m} g^{\beta\delta} g^{\gamma\epsilon}(\partial_\delta g_{\epsilon\alpha} - \partial_\epsilon g_{\delta\alpha} + \partial_\alpha g_{\delta\epsilon} ) \Pi_\beta \Pi_\gamma + \frac{q}{m} F_{\alpha\beta} g^{\beta\gamma} \Pi_\gamma \\
&= \frac{1}{2m} g^{\beta\delta} g^{\gamma\epsilon}(\partial_\delta g_{\epsilon\alpha} + \partial_\alpha g_{\delta\epsilon} - \partial_\epsilon g_{\alpha\delta}  ) \Pi_\beta \Pi_\gamma + \frac{q}{m} F_{\alpha\beta} g^{\beta\gamma} \Pi_\gamma \\
&= \frac{1}{m} g^{\beta\delta} \Gamma^\gamma_{\delta\alpha} \Pi_\beta \Pi_\gamma + \frac{q}{m} F_{\alpha\beta} g^{\beta\gamma} \Pi_\gamma \\
&= d_sx^\delta \Gamma^\gamma_{\delta\alpha} \Pi_\gamma + \frac{q}{m} F_{\alpha\beta} g^{\beta\gamma} \Pi_\gamma \\
D_s \Pi_\alpha &= d_s \Pi_\alpha - d_sx^\delta \Gamma^\gamma_{\delta\alpha} \Pi_\gamma = \frac{q}{m} F_{\alpha\beta} g^{\beta\gamma} \Pi_\gamma \\
d_s f(x^\alpha) =\{f(x^\alpha), \mathcal{H}\} &= \frac{1}{2m} \{f(x^\alpha), \Pi_\beta g^{\beta\gamma} \Pi_\gamma\} \\
&= \frac{1}{m} \Pi_\beta g^{\beta\gamma} \{f(x^\alpha), \Pi_\gamma\} = g_{\beta\delta} d_s x^\delta g^{\beta\gamma} \partial_\gamma f(x^\alpha) \\
&= d_s x^\delta \partial_\delta f(x^\alpha) = d_s f(x^\alpha) \\
\end{aligned}
\end{equation}

\section{Position and velocity}

\begin{equation}
\begin{aligned}
q^\alpha &= x^\alpha \\
p_\alpha &= m g_{\alpha \beta} u^\beta + q A_\alpha \\
\mathcal{H} &= \frac{1}{2} m u^\alpha g_{\alpha\beta} u^\beta \\
e^{q^\alpha} &= \frac{\partial q^\alpha}{\partial x^\beta}e^{x^\beta} + \frac{\partial q^\alpha}{\partial u^\gamma}e^{u^\gamma} = e^{x^\alpha} \\
e^{p_\alpha} &= \frac{\partial p_\alpha}{\partial x^\beta}e^{x^\beta} + \frac{\partial p_\alpha}{\partial u^\gamma}e^{u^\gamma} \\
&= \left(m \frac{\partial g_{\alpha\gamma}}{\partial x^\beta} u^\gamma + q \frac{\partial A_\alpha}{\partial x^\beta} \right)e^{x^\beta} + m g_{\alpha \gamma} e^{u^\gamma} \\
\theta &= (m g_{\alpha \beta} u^\beta + q A_\alpha) e^{x^\alpha} \\
\omega &= e^{x^\alpha} \wedge \left[ \left(m \frac{\partial g_{\alpha\gamma}}{\partial x^\beta} u^\gamma + q \frac{\partial A_\alpha}{\partial x^\beta} \right)e^{x^\beta} + m g_{\alpha \gamma} e^{u^\gamma} \right] \\
&= \left(m \frac{\partial g_{\alpha\gamma}}{\partial x^\beta} u^\gamma + q \frac{\partial A_\alpha}{\partial x^\beta} \right) e^{x^\alpha} \wedge e^{x^\beta} + m g_{\alpha \gamma} e^{x^\alpha} \wedge e^{u^\gamma} \\
&= \left(m u^\gamma \left( \frac{\partial g_{\alpha\gamma}}{\partial x^\beta} -  \frac{\partial g_{\beta\gamma}}{\partial x^\alpha}\right) + q \left( \frac{\partial A_\alpha}{\partial x^\beta} - \frac{\partial A_\beta}{\partial x^\alpha}\right) \right) e^{x^\alpha} \otimes e^{x^\beta} \\
&+ m g_{\alpha \gamma} e^{x^\alpha} \otimes e^{u^\gamma} - m g_{\alpha \gamma} e^{u^\gamma} \otimes e^{x^\alpha} \\
F_{\alpha\beta} &= \partial_\alpha A_\beta - \partial_\beta A_\alpha \\
G_{\alpha\beta\gamma} &= \partial_\alpha g_{\beta \gamma} - \partial_\beta g_{\alpha \gamma} = \frac{1}{2} (\partial_\alpha g_{\beta \gamma} - \partial_\beta g_{\alpha \gamma}) - \frac{1}{2} (\partial_\beta g_{\alpha \gamma} - \partial_\alpha g_{\beta \gamma}) \\
&= \frac{1}{2} (\partial_\gamma g_{\alpha \beta} + \partial_\alpha g_{\beta \gamma} - \partial_\beta g_{\alpha \gamma}) - \frac{1}{2} (\partial_\gamma g_{\alpha \beta} + \partial_\beta g_{\alpha \gamma} - \partial_\alpha g_{\beta \gamma}) \\
&= \Gamma_{\beta\alpha\gamma} - \Gamma_{\alpha\beta\gamma} \\
\omega_{ab} &= \left[ \begin{matrix}
- m G_{\alpha\beta\gamma} u^\gamma - q F_{\alpha\beta} & mg_{\alpha \beta} \\[2.2ex]
- mg_{\alpha \beta} & 0 \end{matrix} \right] \\
\end{aligned}
\end{equation}
\begin{equation}
\begin{aligned}
G^{\alpha\beta\gamma} &= g^{\alpha\delta}g^{\beta\epsilon}g^{\gamma\zeta} G_{\delta\epsilon\zeta} = g^{\alpha\delta}g^{\beta\epsilon}g^{\gamma\zeta} \partial_\delta g_{\epsilon\zeta} - g^{\alpha\delta}g^{\beta\epsilon}g^{\gamma\zeta} \partial_\epsilon g_{\delta\zeta}\\
&= - g^{\alpha\delta} \partial_\alpha g^{\beta\gamma} + g^{\beta\epsilon} \partial_\beta g^{\alpha\gamma} \\
&= \partial^\beta g^{\alpha\gamma} - \partial^\alpha g^{\beta\gamma} \\
F^{\alpha\beta} &= g^{\alpha\gamma}g^{\beta\delta} F_{\gamma\delta} = g^{\alpha\gamma}g^{\beta\delta} \partial_\gamma A_{\delta} - g^{\alpha\gamma}g^{\beta\delta} \partial_\delta A_{\gamma}  \\
&= g^{\alpha\gamma} \partial_\gamma (g^{\beta\delta} A_{\delta}) - g^{\beta\delta} \partial_\delta ( g^{\alpha\gamma}A_{\gamma}) - g^{\alpha\gamma} \partial_\gamma g^{\beta\delta} A_{\delta} + g^{\beta\delta} \partial_\delta g^{\alpha\gamma}A_{\gamma}\\
&= \partial^\alpha A^\beta - \partial^\beta A^\alpha + \partial ^\beta g^{\alpha \gamma} A_\gamma - \partial^\alpha g^{\beta \delta} A_\delta\\
&= \partial^\alpha A^\beta - \partial^\beta A^\alpha +G^{\alpha\beta\gamma} A_\gamma
\end{aligned}
\end{equation}
\begin{equation}
\begin{aligned}
\partial \omega &= \partial \left(\left(m \partial_\beta g_{\alpha \gamma}u^\gamma + q \partial_\beta A_\alpha\right)e^{x^\alpha}\wedge e^{x^\beta} + mg_{\alpha\beta} e^{x^\alpha}\wedge e^{u^\beta}\right) \\ 
&= \partial_{x^\delta} \left(m \partial_\beta g_{\alpha \gamma}u^\gamma + q \partial_\beta A_\alpha\right)e^{x^\delta}\wedge e^{x^\alpha}\wedge e^{x^\beta} + m \partial_{x^\delta}  g_{\alpha\beta} e^{x^\delta}\wedge e^{x^\alpha}\wedge e^{u^\beta} \\
&+ \partial_{u^\delta} \left(m \partial_\beta g_{\alpha \gamma}u^\gamma + q \partial_\beta A_\alpha\right)e^{u^\delta}\wedge e^{x^\alpha}\wedge e^{x^\beta} + m \partial_{u^\delta} g_{\alpha\beta} e^{u^\delta}\wedge  e^{x^\alpha}\wedge e^{u^\beta} \\
&= \left(m \partial_\delta \partial_\beta g_{\alpha \gamma}u^\gamma + q \partial_\delta \partial_\beta A_\alpha\right)e^{x^\delta}\wedge e^{x^\alpha}\wedge e^{x^\beta} + m \partial_\delta  g_{\alpha\beta} e^{x^\delta}\wedge e^{x^\alpha}\wedge e^{u^\beta} \\
&+ m \partial_\beta g_{\alpha \gamma}\delta^\gamma_\delta e^{u^\delta}\wedge e^{x^\alpha}\wedge e^{x^\beta}  \\
&= \left(m \partial_\delta \partial_\beta g_{\alpha \gamma}u^\gamma + q \partial_\delta \partial_\beta A_\alpha\right)e^{x^\delta}\wedge e^{x^\alpha}\wedge e^{x^\beta} + m \partial_\delta  g_{\alpha\beta} e^{x^\delta}\wedge e^{x^\alpha}\wedge e^{u^\beta} \\
&+ m \partial_\delta g_{\alpha \beta} e^{u^\beta}\wedge e^{x^\alpha}\wedge e^{x^\delta}  \\
&= \left(m \partial_\delta \partial_\beta g_{\alpha \gamma}u^\gamma + q \partial_\delta \partial_\beta A_\alpha\right)e^{x^\delta}\wedge e^{x^\alpha}\wedge e^{x^\beta} + m \partial_\delta  g_{\alpha\beta} e^{x^\delta}\wedge e^{x^\alpha}\wedge e^{u^\beta} \\
&- m \partial_\delta g_{\alpha \beta} e^{x^\delta}\wedge e^{x^\alpha}\wedge e^{u^\beta} \\
\end{aligned}
\end{equation}
\begin{equation}
\begin{aligned}
\{x^\alpha, x^\beta\} &= \{q^\alpha, q^\beta\} = 0 \\
\{x^\alpha, u^\beta\} &= \{q^\alpha, \frac{1}{m} g^{\beta\gamma}(p_\gamma - q A_\gamma)\} = \{q^\alpha, \frac{1}{m} g^{\beta\gamma} p_\gamma\} - \{q^\alpha, \frac{q}{m} g^{\beta\gamma} A_\gamma\} \\
&= \frac{1}{m} g^{\alpha\beta} \\
\{u^\alpha, u^\beta\} &= \frac{1}{m^2} \{g^{\alpha \gamma} p_\gamma - q A^\alpha, g^{\beta \delta} p_\delta - q A^\beta\} \\
&= \frac{1}{m^2}\left[ \{g^{\alpha \gamma} p_\gamma, g^{\beta \delta} p_\delta\} - \{g^{\alpha \gamma} p_\gamma, q A^\beta\} - \{q A^\alpha , g^{\beta \delta} p_\delta \} + \{q A^\alpha , q A^\beta\} \right]\\
&= \frac{1}{m^2}\left[ g^{\alpha \gamma} \{p_\gamma, p_\delta\} g^{\beta \delta} + p_\gamma \{g^{\alpha \gamma}, p_\delta\} g^{\beta \delta} + g^{\alpha \gamma} \{p_\gamma, g^{\beta \delta}\} p_\delta + p_\gamma \{g^{\alpha \gamma}, g^{\beta \delta}\} p_\delta \right.\\
&\left. - g^{\alpha \gamma} \{p_\gamma, q A^\beta\} - p_\gamma \{g^{\alpha \gamma} , q A^\beta\} - \{q A^\alpha , p_\delta \} g^{\beta \delta} - \{q A^\alpha , g^{\beta \delta} \} p_\delta \right]\\
&= \frac{1}{m^2}\left[ G^{\alpha\beta\gamma} p_\gamma  + q (\partial^\alpha A^\beta - \partial^\beta A^\alpha) \right] \\
&= \frac{1}{m^2}\left[ G^{\alpha \beta \gamma} m ( g_{\gamma \delta} u^\delta + q A_\gamma ) + q (\partial^\alpha A^\beta - \partial^\beta A^\alpha) \right] \\
&= \frac{1}{m^2}\left[ G^{\alpha \beta \gamma} m g_{\gamma \delta} u^\delta + q (G^{\alpha \beta \gamma} A_\gamma + \partial^\alpha A^\beta - \partial^\beta A^\alpha) \right] \\
&= \frac{1}{m^2}\left[ G^{\alpha \beta \gamma} m g_{\gamma \delta} u^\delta +  q F^{\alpha \beta} \right] \\
\end{aligned}
\end{equation}
\begin{equation}
\begin{aligned}
d_s x^\alpha = \{x^\alpha, \mathcal{H}\} &= \frac{1}{2} m  \{x^\alpha, u^\beta g_{\beta\gamma} u^\gamma\} = m u^\beta g_{\beta \gamma} \{x^\alpha, u^\gamma\}\\
&= m u^\beta g_{\beta\gamma} \frac{1}{m} g^{\alpha\gamma} = u^\alpha \\
d_s u^\alpha = \{ u^\alpha , \mathcal{H} \} &= \frac{1}{2} m \{u^\alpha, u^\beta g_{\beta\gamma} u^\gamma\} \\
&=  m u^\beta g_{\beta\gamma} \{u^\alpha,  u^\gamma\} + \frac{1}{2} m u^\beta u^\gamma \{u^\alpha,  g_{\beta\gamma} \} \\
&= m u^\beta g_{\beta\gamma} \frac{1}{m^2} (G^{\alpha \gamma \delta} m g_{\delta \epsilon} u^\epsilon +  q F^{\alpha \gamma}) - \frac{1}{2} m u^\beta u^\gamma \frac{1}{m} g^{\alpha \delta} \partial_\delta g_{\beta\gamma} \\
&= u^\beta u^\epsilon g_{\beta\gamma} g_{\epsilon \delta} G^{\alpha \gamma \delta} - \frac{1}{2} u^\beta u^\gamma g^{\alpha \delta} \partial_\delta g_{\beta\gamma} + \frac{q}{m} F^{\alpha \gamma}g_{\gamma\beta}u^\beta \\
&= u^\beta u^\epsilon g^{\alpha\gamma} G_{\gamma \beta \epsilon} - \frac{1}{2} u^\beta u^\gamma g^{\alpha \delta} (\partial_\beta g_{\gamma\delta} - \partial_\beta g_{\gamma\delta} + \partial_\delta g_{\beta\gamma}) + \frac{q}{m} F^{\alpha \gamma}g_{\gamma\beta}u^\beta \\
&= u^\beta u^\gamma g^{\alpha\delta} G_{\delta \beta \gamma} -  u^\beta u^\gamma g^{\alpha \delta} \frac{1}{2} (\partial_\gamma g_{\delta\beta} + \partial_\delta g_{\beta\gamma} - \partial_\beta g_{\gamma\delta}) + \frac{q}{m} F^{\alpha \gamma}g_{\gamma\beta}u^\beta \\
&= u^\beta u^\gamma g^{\alpha\delta} (\Gamma_{\beta \delta \gamma} - \Gamma_{\delta \beta \gamma} - \Gamma_{\beta \delta \gamma}) + \frac{q}{m} F^{\alpha \gamma}g_{\gamma\beta}u^\beta \\
&= - u^\beta u^\gamma g^{\alpha\delta} \Gamma_{\delta \beta \gamma} + \frac{q}{m} F^{\alpha \gamma}g_{\gamma\beta}u^\beta \\
D_s u^\alpha &= d_s u^\alpha + u^\beta d_sx^\gamma \Gamma^\alpha_{\beta\gamma} = \frac{q}{m} F^{\alpha \gamma}g_{\gamma\beta}u^\beta \\
\end{aligned}
\end{equation}

\section{Anti-symmetric covariant derivative}
\begin{equation}
\begin{aligned}
\nabla_\alpha A_\beta &= \partial_\alpha A_\beta - \Gamma^\gamma_{\beta\alpha} A_\gamma  \\
\nabla_\alpha A_\beta - \nabla_\beta A_\alpha &= \partial_\alpha A_\beta - \Gamma^\gamma_{\beta\alpha} A_\gamma -\partial_\beta A_\alpha + \Gamma^\gamma_{\alpha\beta} A_\gamma  \\
&= \partial_\alpha A_\beta -\partial_\beta A_\alpha  \\
\nabla_\alpha A^\beta &= \partial_\alpha A^\beta + \Gamma^\beta_{\gamma\alpha} A^\gamma  \\
\nabla_\alpha A_\beta = \nabla_\alpha ( g_{\beta\gamma} A^\gamma) &= g_{\beta\gamma} \nabla_\alpha A^\gamma = g_{\beta\gamma} \partial_\alpha A^\gamma + g_{\beta\gamma} \Gamma^\gamma_{\delta\alpha} A^\delta \\
&= \partial_\alpha (g_{\beta\gamma} A^\gamma) - \partial_\alpha g_{\beta\gamma} A^\gamma + g_{\beta\gamma} \Gamma^\gamma_{\delta\alpha} A^\delta \\
&= \partial_\alpha A_\beta - \partial_\alpha g_{\beta\gamma} A^\gamma +  \Gamma_{\beta\gamma\alpha} A^\gamma \\
&= \partial_\alpha A_\beta - \partial_\alpha g_{\beta\gamma} A^\gamma +  \frac{1}{2} (\partial_\alpha g_{\beta\gamma} + \partial_\gamma g_{\beta\alpha} - \partial_\beta g_{\alpha\gamma}) A^\gamma \\
&= \partial_\alpha A_\beta +  \frac{1}{2} ( - \partial_\alpha g_{\beta\gamma} + \partial_\gamma g_{\beta\alpha} - \partial_\beta g_{\alpha\gamma}) A^\gamma \\
&= \partial_\alpha A_\beta - \Gamma_{\gamma\beta\alpha} A^\gamma \\
&= \partial_\alpha A_\beta - \Gamma^\gamma_{\beta\alpha} A_\gamma = \nabla_\alpha A_\beta \\
\nabla^\alpha A^\beta - \nabla^\beta A^\alpha &= g^{\alpha\gamma} \nabla_\gamma A^\beta - g^{\beta\gamma} \nabla_\gamma A^\alpha \\
&= g^{\alpha\gamma} (\partial_\gamma A^\beta + \Gamma^\beta_{\delta\gamma} A^\delta) - g^{\beta\gamma} (\partial_\gamma A^\alpha + \Gamma^\alpha_{\delta\gamma} A^\delta) \\
&= \partial^\alpha A^\beta - \partial^\beta A^\alpha + g^{\alpha\delta} g^{\beta\epsilon} A^\gamma( \Gamma_{\epsilon\delta\gamma} - \Gamma_{\delta\epsilon\gamma}) \\
&= \partial^\alpha A^\beta - \partial^\beta A^\alpha + G^{\alpha\beta\gamma} A_\gamma \\
\end{aligned}
\end{equation}



\begin{thebibliography}{0}
	
\end{thebibliography}

\end{document}
